src/cbor/pulse/raw/CBOR.Pulse.API.Det.C.fst
@@ -3,6 +3,111 @@ module CBOR.Pulse.API.Det.C
 (* NOTE: this .fst file does not need anything from the Raw namespace,
 but it has been moved here to be hidden from verified clients. *)
 
+module SU = Pulse.Lib.Slice.Util
+
+```pulse
+fn cbor_det_validate
+  (input: AP.ptr U8.t)
+  (input_len: SZ.t)
+  (#pm: perm)
+  (#v: Ghost.erased (Seq.seq U8.t))
+requires
+    (pts_to input #pm v ** pure (SZ.v input_len == Seq.length v))
+returns res: SZ.t
+ensures
+    (pts_to input #pm v ** pure (
+      cbor_det_validate_post v res
+    ))
+{
+  let s = SU.arrayptr_to_slice_intro_trade input input_len;
+  let res = CBOR.Pulse.API.Det.Common.cbor_det_validate s;
+  Trade.elim _ (pts_to input #pm v);
+  res
+}
+```
+
+module ID = FStar.IndefiniteDescription
+
+let cbor_det_validate_success_elim
+  (len: SZ.t)
+  (v: Seq.seq U8.t)
+: Pure (Ghost.erased (Spec.cbor & Seq.seq U8.t))
+    (requires exists v1 v2 . Ghost.reveal v == Spec.cbor_det_serialize v1 `Seq.append` v2 /\ SZ.v len == Seq.length (Spec.cbor_det_serialize v1))
+    (ensures fun (v1, v2) ->
+      Ghost.reveal v == Spec.cbor_det_serialize v1 `Seq.append` v2 /\ SZ.v len == Seq.length (Spec.cbor_det_serialize v1)
+    )
+= let p v1 v2 = Ghost.reveal v == Spec.cbor_det_serialize v1 `Seq.append` v2 /\ SZ.v len == Seq.length (Spec.cbor_det_serialize v1) in
+  assert (exists v1 v2 . p v1 v2);
+  let v1 = FStar.IndefiniteDescription.indefinite_description_tot _ (fun v1 -> exists v2 . p v1 v2) in
+  assert (exists v2 . p v1 v2);
+  let v2 = FStar.IndefiniteDescription.indefinite_description_tot _ (fun v2 -> p v1 v2) in
+  (Ghost.reveal v1, Ghost.reveal v2)
+
+```pulse
+fn cbor_det_parse
+  (input: AP.ptr U8.t)
+  (len: SZ.t)
+  (#pm: perm)
+  (#v: Ghost.erased (Seq.seq U8.t))
+requires
+    (pts_to input #pm v ** pure (
+      exists v1 v2 . Ghost.reveal v == Spec.cbor_det_serialize v1 `Seq.append` v2 /\ SZ.v len == Seq.length (Spec.cbor_det_serialize v1)
+    ))
+returns res: cbor_det_t
+ensures
+    (exists* v' .
+      cbor_det_match 1.0R res v' **
+      Trade.trade (cbor_det_match 1.0R res v') (pts_to input #pm v) ** pure (
+        SZ.v len <= Seq.length v /\
+        Seq.slice v 0 (SZ.v len) == Spec.cbor_det_serialize v'
+    ))
+{
+  let v1v2 = cbor_det_validate_success_elim len v;
+  assert (pure (Seq.equal (Seq.slice v 0 (SZ.v len)) (Spec.cbor_det_serialize (fst v1v2))));
+  let gr : Ghost.erased (AP.ptr U8.t) = AP.ghost_split input len;
+  ghost fn aux (_: unit)
+  requires pts_to (Ghost.reveal gr) #pm (Seq.slice v (SZ.v len) (Seq.length v)) ** pts_to input #pm (Seq.slice v 0 (SZ.v len))
+  ensures pts_to input #pm v
+  {
+    Seq.lemma_split v (SZ.v len);
+    AP.join input gr
+  };
+  Trade.intro _ _ _ aux;
+  Seq.append_empty_r (Spec.cbor_det_serialize (fst v1v2));
+  let s = SU.arrayptr_to_slice_intro_trade input len;
+  Trade.trans _ _ (pts_to input #pm v);
+  S.pts_to_len s;
+  let res = CBOR.Pulse.API.Det.Common.cbor_det_parse s len;
+  Trade.trans _ _ (pts_to input #pm v);
+  res
+}
+```
+
+#restart-solver
+```pulse
+fn cbor_det_serialize
+  (x: cbor_det_t)
+  (output: AP.ptr U8.t)
+  (output_len: SZ.t)
+  (#y: Ghost.erased Spec.cbor)
+  (#pm: perm)
+requires
+    (exists* v . cbor_det_match pm x y ** pts_to output v ** pure (SZ.v output_len == Seq.length v /\ Seq.length (Spec.cbor_det_serialize y) <= SZ.v output_len))
+returns res: SZ.t
+ensures
+    (exists* v . cbor_det_match pm x y ** pts_to output v ** pure (
+      cbor_det_serialize_postcond y res v
+    ))
+{
+  let ou = S.arrayptr_to_slice_intro output output_len;
+  S.pts_to_len ou;
+  let res = CBOR.Pulse.API.Det.Common.cbor_det_serialize x ou;
+  assert (pure (SZ.v res == Seq.length (Spec.cbor_det_serialize y)));
+  S.arrayptr_to_slice_elim ou;
+  res
+}
+```
+
 ```pulse
 fn cbor_det_mk_string_from_array (_: unit) : cbor_det_mk_string_from_array_t
 =
@@ -89,6 +194,22 @@ fn cbor_det_mk_map_from_array (_: unit) : cbor_det_mk_map_from_array_t
   Trade.intro _ _ _ aux;
   Trade.reg_r (pts_to s va') (A.pts_to a va') (PM.seq_list_match va vv (cbor_det_map_entry_match pv));
   Trade.trans (cbor_det_match p' res (Spec.pack (Spec.CMap v'))) _ _;
+  res
+}
+```
+
+```pulse
+fn cbor_det_get_string
+  (_: unit)
+: cbor_det_get_string_t
+=
+  (x: _)
+  (#p: _)
+  (#y: _)
+{
+  let sl = CBOR.Pulse.API.Det.Common.cbor_det_get_string () x;
+  let res = SU.slice_to_arrayptr_intro_trade sl;
+  Trade.trans _ _ (cbor_det_match p x y);
   res
 }
 ```
